
# Bonus Topic: The Lambda Calculus

![](figures/xkcd_excel.png)

# Intro: `python` lambdas

- In many languages, a "lambda" function is a function that can
    be treated like an object (usually with captured variables)
- However, `python` has a different interpretation!

```py
a = lambda x: x ** 2
print(a(5))
# >> 25

plus = lambda lhs: lambda rhs: lhs + rhs
print(plus(123)(321))
# >> 444
```

- **Generally:** `lambda b: f(b)` is a formula which, when
    applied on input $x$, returns $f(x)$
    - $b$ is the thing that will be replaced
    - Everything after the colon is the text in which $b$ will
        be replaced

# Church's Version

- Alonzo Church was Turing's PhD advisor at Princeton
- Followed the work of GÃ¶del, Peano, Principia Mathematica in
    formalizing mathematics
- Also following the string-rewriting-rule formalizations of
    Thue
- He invented "the lambda calculus", or $\lambda$-calculus

**Def:** $\lambda$-calculus. Let $M[x := N]$ mean "string $M$,
but with any occurrence of $x$ replaced with $N$".

1. $\lambda x . M$ is a **lambda abstraction**
2. If $M$ is a lambda abstraction, $M N$ is an **application**
3. $\lambda x . M$ and $\lambda y . M[x := y]$ are equivalent
    ($\alpha$-conversion, used to avoid collisions)
4. $(\lambda x . M)(N) = M[x := N]$ is the result of an
    application ($\beta$-reduction, represents computation)

# Example

**Ex:** $(\lambda x . \sqrt{x})((\lambda x . x^2)5)$

1. Input: $(\lambda x . \sqrt{x})((\lambda x . x^2)5)$
2. $\beta$-reduction: $\sqrt{((\lambda x . x^2)5)}$
3. $\beta$-reduction: $\sqrt{5^2}$
4. Arithmetic: $5$

# Currying

- What if we want to have multiple arguments?
- In `python`, `lambda x, y: f(x, y)` is legal
    - This is **not** legal in $\lambda$-calculus!
    - However, abstractions are allowed to return abstractions!
- We can make a function that takes the first argument and
    returns a function taking the second argument

```python
mean = lambda a: lambda b: lambda c: (a + b + c) / 3

# mean(1) is `lambda b: lambda c: (1 + b + c) / 3`
# mean(1)(2) is `lambda c: (1 + 2 + c) / 3`
# mean(1)(2)(3) is `(1 + 2 + 3) / 3`

print(mean(1)(2)(3))
# >> 2
```

- This is called **Currying**
- Named after Haskell Curry (also the namesake of the Haskell
    language)

# Currying Example

**Ex:**
$[\lambda x.\lambda y.\lambda z.\frac{x}{y}+z](15)(3)(37)$

1. Input:
    $[\lambda x.\lambda y.\lambda z.\frac{x}{y}+z](15)(3)(37)$
2. $\beta$-reduction:
    $[\lambda y.\lambda z.\frac{15}{y}+z](3)(37)$
3. $\beta$-reduction: $[\lambda z.\frac{15}{3}+z](37)$
4. $\beta$-reduction: $\frac{15}{3}+37$
5. Arithmetic: $\frac{15}{3} + 37 = 5 + 37 = 42$

![](figures/xkcd_currying.png)

# The $Y$-Combinator

Consider the classical "paradox" discovered by Curry:

$$
Y = \lambda f . (\lambda x . f(x x))(\lambda x . f(x x))
$$

**Puzzle: What does $Y g$ $\beta$-reduce to?**

# $Y$-Combinator $\beta$-reduction

1. $Y g$ (input)
2. $= \lambda f . (\lambda x . f(x x))(\lambda x . f(x x)) g$
    (by definition of $Y$)
3. $= (\lambda x . g(x x)) (\lambda x . g(x x))$
    (by $\beta$-reduction)
4. $= g((\lambda x . g(x x)) (\lambda x . g(x x)))$
    (by $\beta$-reduction)
5. $= g(Y g)$ (by equivalency of steps 1 and 3)
6. $= g(g(Y g)) = g(g(g(Y g))) = \ldots$ (ad infinitum)

This can be used to create loops in $\lambda$-calculus!

# Turing-Equivalency

- Church and Turing proved $\lambda$-calculus is equivalent to
    Turing machines
- Since both Peano arithmetic and $\lambda$-calculus are
    Turing-equivalent, they must be equivalent to each other!
    - They are both equally valid characterizations of unbounded
        arithmetic on the natural numbers
